Split scripts (#1)
* copy Holmakefile

* commit

* copy Holmakefile

* commit

* Delete baseScript.sml

* Delete chainScript.sml

* Update README.md

* Update README.md

* Update README.md

* Update README.md

higher-order/baseScript.sml
@@ -16,56 +16,15 @@
     THEOREMS
     GOALTHMS
    +----------------------------------------------------------------------------+ *)
-
 (*START ------------------------------------------------------------------------- *)
 app load ["stringTheory","wordsTheory", "llistTheory"(* , "preamble" *)];
 
-open arithmeticTheory listTheory stringTheory wordsTheory combinTheory pred_setTheory relationTheory prim_recTheory HolKernel boolLib Parse bossLib optionTheory llistTheory ;
+open arithmeticTheory listTheory stringTheory combinTheory wordsTheory HolKernel boolLib Parse bossLib optionTheory llistTheory;
+
+open sc1TypesTheory
+open chainTheory
 
 val _ = new_theory "base";
-
-(*DEFINITIONS ------------------------------------------------------------------- *)
-Datatype:
-    Negotiation = NotSet | WaitingCustomer | WaitingSupplier | NegotiationRejected | NegotiationApproved ;
-    PaymentStatus = WaitingForPayment | PaymentCompleted | PaymentRejected ;
-    Phase = PhaseAgreement | PhaseTasks | PhaseDeclined ;
-    TaskStatus = TaskNotAccepted | TaskAccepted | TaskReadyToPerform | GasRequested | Performing | Confirmed | TaskCompleted ;
-    PaymentType = Pre | Post | Delayed
-End
-
-Datatype:
-    Person = <|id:num; name:string|>;
-    AgreementDetails = <|details:string; bankAddress:num|>;
-    Agreement = <|negotiation:Negotiation; customer:Person; supplier:Person; details:AgreementDetails|>;
-    PriceChange = <|price:num; negotiation:Negotiation; startTime:num|>;
-    PaymentOrder = <|amount:num; paymentTime:num; paymentId:num; taskId:num; paymentStatus:PaymentStatus; direction:bool|>;
-    Task = <|taskID:num; negotiation:Negotiation; captain:Person; worker:Person; expectedGas:num; requestedGas:num; suppliedGas:num; totalGas:num; requestTime:num; suppliedTime:num; completionTime:num; paymentTime:num; taskStatus:TaskStatus; paymentType:PaymentType|>;
-    Campaign = <|agreement:Agreement; tasks:Task list; negotiation:Negotiation; priceChanges:PriceChange list; phase:Phase; paymentOrders:PaymentOrder list|>;
-End
-
-Datatype:
-    SCType = TypeInt | TypeString | TypeBool | TypeAgreement | TypeTask | TypeNegotiation | TypePriceChange | TypePaymentOrder | TypeCampaign | TypePerson  | TypeList  | TypePaymentStatus | TypeAgreementDetails  | TypeTaskStatus  | TypePaymentType | TypePhase
-End
-
-Datatype:
-    SCvalue = SCInt num | SCString string | SCBool bool | SCAgreement Agreement | SCTask Task | SCNegotiation Negotiation | SCPriceChange PriceChange | SCPaymentOrder PaymentOrder | SCCampaign Campaign | SCPerson Person | SCPaymentStatus PaymentStatus  | SCTaskStatus TaskStatus  | SCAgreementDetails AgreementDetails  | SCPaymentType PaymentType | SCPhase Phase
-End
-
-Datatype:
-    Context = <|msgSender:num; blockNum:num|>
-End
-
-Datatype:
-    optionErr = Some 'a | Ret 'a 'a | None string
-End
-
-Datatype:
-    optErrSC = Some' SCvalue | None' string
-End
-
-Datatype:
-  returnType = <| state : Campaign; value : optErrSC |>
-End
 
 val const_defs = [
     Define `BAD_ERR = None "Error"`,
@@ -113,7 +72,6 @@ val const_defs = [
     Define `WRNG_COND_015 = None "Wrong conditions. Please, check: sender is Worker, Task is approved and performing now."`,
     Define `WRNG_COND_016 = None "Wrong conditions. Please, check: params are two numbers, phase is PhaseTasks, Agreement is approved, at least one PriceChange is approved."`
     ];
-
 
 (*BASICS ------------------------------------------------------------------------ *)
 
@@ -1224,7 +1182,6 @@ Definition constructor_def:
       customer_id customer_name supplier_id supplier_name agreement_details bank_addr
 End
 
-
 val _ = map type_of [``getAgreement_typed``, ``rejectAgreement_typed``, ``approveAgreement_typed``, ``changeAgreement_typed``, ``getPriceChangeWithNumber_typed``, ``getPriceChangesLength_typed``, ``rejectPrice_typed``, ``approvePrice_typed``, ``declinePrice_typed``, ``createPriceChange_typed``, ``getTask_typed``, ``approveTask_typed``, ``rejectTask_typed``, ``acceptTask_typed``, ``removeTask_typed``, ``addTask_typed``, ``readyToPerformTask_typed``, ``requestGas_typed``, ``completePayment_typed``, ``performTask_typed``, ``completeTask_typed``, ``confirmTask_typed``];
 
 Definition chooseFunction_def:
@@ -1259,212 +1216,6 @@ execute f context (params:SCvalue list) campaign =
   case (chooseFunction f) of
     SOME func => func context params campaign
   | NONE      => NEX_function
-End
-
-
-(* model *)
-
-Type State = “:SCvalue optionErr”;
-
-Datatype:
-    Address = Contract_address num | Client_address num
-End
-
-Definition take_address_def:
-  take_address (Contract_address n) = n ∧
-  take_address (Client_address n) = n
-End
-
-Definition address_is_contract_def:
-  address_is_contract (Contract_address num) = T ∧
-  address_is_contract (Client_address num) = F
-End
-
-(* информация о блокчейне для контракта *)
-Datatype:
-  Chain = <| chainHeight : num; blockNum : num|>
-End
-
-Definition get_chainHeight_def:
-  get_chainHeight = Chain_chainHeight
-End
-
-Definition get_blockNum_def:
-  get_blockNum = Chain_blockNum
-End
-
-Definition ChainEquiv_def:
-    ChainEquiv c1 c2 = ((get_chainHeight c1 = get_chainHeight c2) ∧
-    (get_blockNum c1 = get_blockNum c2))
-End
-
-(* информация о запросе, который привел к исполнению контракта *)
-Datatype :
-  ContractCallContext = <| msgSender : Address; ctxContractAddress : Address|>
-End
-
-Definition get_msgSender_def:
-  get_msgSender = ContractCallContext_msgSender
-End
-
-Definition get_ctxContractAddress_def:
-  get_ctxContractAddress = ContractCallContext_ctxContractAddress
-End
-
-Datatype :
-  Data = <|functionSignature: num; params: SCvalue list |>
-End
-
-Definition get_functionSignature_def:
-  get_functionSignature = Data_functionSignature
-End
-
-Definition get_params_def:
-  get_params = Data_params
-End
-
-Datatype :
-  Setup = <|code: word8 list; setupParams: SCvalue list |>
-End
-
-Definition get_setupparams_def:
-  get_setupparams = Setup_setupParams
-End
-
-Datatype : 
-  Contract = <| init: (Chain -> ContractCallContext -> Setup -> State); receive: (Chain -> ContractCallContext -> Campaign -> Data -> State) |>
-End
-
-Definition build_context_def :  
-  build_context from n = <| msgSender := from; blockNum := n|>
-End
-
-Definition build_contract_def :  
-  build_contract i r = <| init := i; receive := r|>
-End
-
-Definition get_init_def:
-  get_init = Contract_init
-End
-
-Definition get_receive_def:
-  get_receive = Contract_receive
-End
-
-Datatype:
-  ActionBody = Call Address Data | Deploy Contract Setup | noAct
-End
-
-(* сам запрос к контракту *)
-Datatype :
-  Action = <| actFrom : Address; actBody : ActionBody |> 
-End
-
-Definition get_actFrom_def:
-  get_actFrom = Action_actFrom
-End
-
-Definition get_actBody_def:
-  get_actBody = Action_actBody
-End
-
-Definition act_is_from_account_def: 
-  act_is_from_account act = (address_is_contract (get_actFrom act) = F)
-End
-
-Datatype:
-  Environment = <| envChain : Chain; envContracts : (Address -> Contract option); envContractStates : (Address -> Campaign option)|>
-End
-
-Definition get_envChain_def:
-  get_envChain = Environment_envChain
-End
-
-Definition get_envContracts_def:
-  get_envContracts = Environment_envContracts
-End
-
-Definition get_envContractStates_def:
-  get_envContractStates = Environment_envContractStates
-End
-
-Definition EnvironmentEquiv_def:
-  EnvironmentEquiv e1 e2 = ((ChainEquiv (get_envChain e1) (get_envChain e2)) ∧
-    (∀c. get_envContracts e1 c = get_envContracts e2 c) ∧
-    (∀addr. get_envContractStates e1 addr = get_envContractStates e2 addr))
-End
-
-Definition add_contract_def :  
-  add_contract addr c rec : Environment = 
-    rec with envContracts := (get_envContracts rec) (|addr |-> SOME c|) 
-End
-
-Definition set_contract_state_def :  
-  set_contract_state addr state rec : Environment = 
-    rec with envContractStates := (get_envContractStates rec) (|addr |-> SOME state|) 
-End
-
-Definition build_act_def :  
-  build_act addr body = <| actFrom := addr; actBody := body |>
-End
-
-Definition build_ccc_def :  
-  build_ccc from to= <| msgSender := from; ctxContractAddress := to|>
-End
- 
-Definition get_campaign_def :  
-  get_campaign (Ret (SCCampaign c) _) = SOME c ∧
-  get_campaign (Some (SCCampaign c)) = SOME c ∧
-  get_campaign _ = NONE
-End
-
-Inductive ActionEvaluation:
-      (∀ prevEnv act newEnv from to c setup state. 
-      (address_is_contract to = T) ∧
-      (get_envContracts prevEnv to = NONE) ∧
-      (act = build_act from (Deploy c setup)) ∧
-      (get_campaign (get_init c (get_envChain prevEnv) (build_ccc from to) setup) = SOME state) ∧
-      (newEnv = set_contract_state to state (add_contract to c prevEnv)) ==>
-      ActionEvaluation prevEnv act newEnv) ∧
-      (∀ prevEnv act newEnv from to c prevState data nextState.
-      (get_envContracts prevEnv to = SOME c) ∧
-      (get_envContractStates prevEnv to = SOME prevState) ∧
-      (act = build_act from (Call to data)) ∧
-      (get_campaign (get_receive c (get_envChain prevEnv) (build_ccc from to) prevState data) = SOME nextState) ∧
-      (newEnv = set_contract_state to nextState prevEnv) ==>
-      ActionEvaluation prevEnv act newEnv)
-End
-
-Inductive ChainStep:
-  (∀prevState nextState act. (~(get_actBody act = noAct) ∧
-  ActionEvaluation prevState act nextState) ==> ChainStep prevState nextState)
-End
-
-Inductive ChainedList:
-  (∀ p. ChainedList R p p) ∧
-  (∀ x z. (?y. R x y ∧ ChainedList R y z) ==> ChainedList R x z)  
-End
-
-Inductive ChainTrace :
-  (∀ s1 s2. ChainedList ChainStep s1 s2 ==> ChainTrace s1 s2) 
-End
-
-Definition empty1_def:
-  empty1 _ = NONE
-End
-
-Definition empty2_def:
-  empty2 _ = NONE
-End
-
-Definition emptyState_def:
-  emptyState = <| envChain := <| chainHeight := 0; blockNum := 0|>;
-                  envContracts := empty1;
-                  envContractStates := empty2 |>
-End
-
-Inductive reachable :
-  (∀ s. (ChainTrace emptyState s) ∧ (~ (emptyState = s)) ==> reachable s) 
 End
 
 Definition scReceive_def:
@@ -3093,48 +2844,4 @@ Proof
   STRIP_TAC >> FULL_SIMP_TAC (srw_ss()) [set_contract_state_def, get_envContractStates_def, get_envContracts_def, UPDATE_def]
 QED
 
-Inductive transition_relation:
-  (∀s. transition_relation s s) ∧
-  (∀s t. ChainStep s t ==> transition_relation s t)
-End
-
-Definition invariant_def:
-  invariant p = (!(s: Environment) (t: Environment). p s /\ ChainStep s t ==> p t)  
-End
-
-Definition lAnd_def:
-    lAnd P Q (str : Environment llist) = (P str /\ Q str)
-End
-
-Definition next_def:
-    next P (str : Environment llist) = P (LTL str)
-End
-
-Inductive until:
-    (!(str : Environment llist). Q str ==> until P Q str) ∧
-    (!s (str : Environment llist). P (LCONS s str) /\ until P Q str ==> until P Q (LCONS s str))
-End
-
-CoInductive globally:
-    (globally T) /\
-    (!s (str : Environment llist). P (LCONS s str) /\ globally (P str) ==> globally (P (LCONS s str)))
-End
-
-Definition path_def:
-    path (str : Environment llist) = (globally (transition_relation (THE (LHD str)) (THE (LHD (THE (LTL str))))) /\ 
-                                      (THE (LHD str) = emptyState))
-End
-
-Definition safe_def:
-    safe f = (!str. path str ==> globally (f str))
-End
-
-Definition s2s_def:
-    s2s P (str : Environment llist) = P (THE (LHD str))
-End
-
-Theorem safety:
-    !p e. e = emptyState /\ p e /\ invariant p ==> safe (s2s p)
-Proof 
-    rpt STRIP_TAC >> rw [safe_def, s2s_def] >> fs [invariant_def, path_def] >> rw [Once globally_cases]
-QED
+val _ = export_theory();
