monadic/monadChainScript.sml
@@ -1,0 +1,217 @@
+(*START ------------------------------------------------------------------------- *)
+open preamble
+open basis
+open ml_monad_translator_interfaceLib
+
+open stringTheory
+open wordsTheory
+open listTheory
+open sc1TypesTheory
+     
+val _ = new_theory "monadChain";
+val _ = translation_extends "basisProg";
+val _ = ParseExtras.temp_tight_equality ();
+
+Datatype:
+    Address = Contract_address num | Client_address num
+End
+
+Definition take_address_def:
+  take_address (Contract_address n) = n ∧
+  take_address (Client_address n) = n
+End
+
+Definition address_is_contract_def:
+  address_is_contract (Contract_address num) = T ∧
+  address_is_contract (Client_address num) = F
+End
+
+Datatype :
+  Data = <|functionSignature: num; params: SCvalue list |>
+End
+
+Definition get_functionSignature_def:
+  get_functionSignature = Data_functionSignature
+End
+
+Definition get_params_def:
+  get_params = Data_params
+End
+
+Datatype :
+  Setup = <|code: word8 list; setupParams: SCvalue list |>
+End
+
+Definition get_setupparams_def:
+  get_setupparams = Setup_setupParams
+End
+
+Datatype : 
+  Contract = <| init: (Setup -> State -> (SCvalue, state_exn) exc # State); receive: (Data -> State -> (SCvalue, state_exn) exc # State) |>
+End
+
+Definition build_contract_def :  
+  build_contract i r = <| init := i; receive := r|>
+End
+
+Definition get_init_def:
+  get_init = Contract_init
+End
+
+Definition get_receive_def:
+  get_receive = Contract_receive
+End
+
+Datatype:
+  ActionBody = Call Address Data | Deploy Contract Setup | noAct
+End
+
+(* сам запрос к контракту *)
+Datatype :
+  Action = <| actFrom : Address; actType : ActionBody |> 
+End
+
+Definition get_actFrom_def:
+  get_actFrom = Action_actFrom
+End
+
+Definition get_actType_def:
+  get_actType = Action_actType
+End
+
+Definition act_is_from_account_def: 
+  act_is_from_account act = (address_is_contract (get_actFrom act) = F)
+End
+
+Datatype:
+  Environment = <| envContracts : (Address -> Contract option); envContractStates : (Address -> State option)|>
+End
+
+Definition get_envContracts_def:
+  get_envContracts = Environment_envContracts
+End
+
+Definition get_envContractStates_def:
+  get_envContractStates = Environment_envContractStates
+End
+
+Definition add_contract_def :  
+  add_contract addr c rec : Environment = 
+    rec with envContracts := (get_envContracts rec) (|addr |-> SOME c|) 
+End
+
+Definition set_contract_state_def :  
+  set_contract_state addr state rec : Environment = 
+    rec with envContractStates := (get_envContractStates rec) (|addr |-> SOME state|) 
+End
+
+Definition build_act_def :  
+  build_act addr body = <| actFrom := addr; actType := body |>
+End
+
+Inductive ActionEvaluation:
+      (∀ prevEnv act newEnv from to c setup s0 state. 
+      (address_is_contract to = T) ∧
+      (get_envContracts prevEnv to = NONE) ∧
+      (act = build_act from (Deploy c setup)) ∧
+      (do
+        i <- (get_init c setup);
+        s <- get_state;
+       od s0 = return state s0) ∧
+      (newEnv = set_contract_state to state (add_contract to c prevEnv)) ==>
+      ActionEvaluation prevEnv act newEnv) ∧
+      (∀ prevEnv act newEnv from to c prevState data nextState.
+      (get_envContracts prevEnv to = SOME c) ∧
+      (get_envContractStates prevEnv to = SOME prevState) ∧
+      (act = build_act from (Call to data)) ∧
+      (do
+        r <- (get_receive c data);
+        s <- get_state;
+       od prevState = return nextState prevState) ∧
+      (newEnv = set_contract_state to nextState prevEnv) ==>
+      ActionEvaluation prevEnv act newEnv)
+End
+
+Inductive ChainStep:
+  (∀prevState nextState act. (~(get_actType act = noAct) ∧
+  ActionEvaluation prevState act nextState) ==> ChainStep prevState nextState)
+End
+
+Inductive ChainedList:
+  (∀ p. ChainedList R p p) ∧
+  (∀ x z. (?y. R x y ∧ ChainedList R y z) ==> ChainedList R x z)  
+End
+
+Inductive ChainTrace :
+  (∀ s1 s2. ChainedList ChainStep s1 s2 ==> ChainTrace s1 s2) 
+End
+
+Definition empty1_def:
+  empty1 _ = NONE
+End
+
+Definition empty2_def:
+  empty2 _ = NONE
+End
+
+Definition emptyState_def:
+  emptyState = <| envContracts := empty1;
+                  envContractStates := empty2 |>
+End
+
+Inductive reachable :
+  (∀ s. (ChainTrace emptyState s) ∧ (~ (emptyState = s)) ==> reachable s) 
+End
+
+Inductive transition_relation:
+  (∀s. transition_relation s s) ∧
+  (∀s t. ChainStep s t ==> transition_relation s t)
+End
+
+Definition invariant_def:
+  invariant p = (!(s: Environment) (t: Environment). p s /\ ChainStep s t ==> p t)  
+End
+
+Definition lAnd_def:
+    lAnd P Q (str : Environment llist) = (P str /\ Q str)
+End
+
+Definition next_def:
+    next P (str : Environment llist) = P (LTL str)
+End
+
+Inductive until:
+    (!(str : Environment llist). Q str ==> until P Q str) ∧
+    (!s (str : Environment llist). P (LCONS s str) /\ until P Q str ==> until P Q (LCONS s str))
+End
+
+CoInductive globally:
+    (!s (str : Environment llist). P (LCONS s str) /\ globally (P str) ==> globally (P (LCONS s str)))
+End
+
+Definition path_def:
+    path (str : Environment llist) = (globally (transition_relation (THE (LHD str)) (THE (LHD (THE (LTL str))))) /\ 
+                                      (THE (LHD str) = emptyState))
+End
+
+Definition safe_def:
+    safe f = (!str. path str ==> globally (f str))
+End
+
+Definition s2s_def:
+    s2s P (str : Environment llist) = P (THE (LHD str))
+End
+
+Theorem safety:
+    !p e. e = emptyState /\ p e /\ invariant p ==> safe (s2s p)
+Proof 
+    rw [safe_def, s2s_def] >> fs [invariant_def] >> rw [Once globally_cases] >> fs [path_def] >> fs [Once globally_cases] >> fs [] >> Q.EXISTS_TAC ‘P’ >> Q.EXISTS_TAC ‘s’ >> Q.EXISTS_TAC ‘str''’ >> rw [] >> Q.EXISTS_TAC ‘P’ >> Q.EXISTS_TAC ‘s’ >> Q.EXISTS_TAC ‘str''’ >> rw [] >> fs [Once globally_cases] 
+QED
+
+Theorem globally_induction:
+  !p str. invariant p /\ path str /\ p (THE (LHD str)) ==> globally ((s2s p) str)
+Proof
+  rw [Once globally_cases] >> rw [s2s_def] >> fs [invariant_def, path_def] >> fs [Once globally_cases] >> fs [] >> Q.EXISTS_TAC ‘P’ >> Q.EXISTS_TAC ‘s’ >> Q.EXISTS_TAC ‘str''’ >> rw [] >> Q.EXISTS_TAC ‘P’ >> Q.EXISTS_TAC ‘s’ >> Q.EXISTS_TAC ‘str''’ >> rw [] >> fs [Once globally_cases]
+QED
+
+val _ = export_theory();
